code cleanup

code/experimental/rsa/Division.fst
@@ -15,16 +15,16 @@ module U64 = FStar.UInt64
 
 type bignum = buffer FStar.UInt64.t
 
-type lbytes (len:U32.t) = 
-     b:buffer FStar.UInt64.t{length b = U32.v len} 
+type lbignum (len:U32.t) = 
+     b:bignum{length b = U32.v len} 
 
 type bnlen = (l:U32.t{U32.v l > 0 /\ U32.v l <= 8192})
-type rem_state (rLen:bnlen) (modLen:bnlen) = lbytes U32.(rLen +^ rLen +^ modLen +^ modLen)
+type rem_state (rLen:bnlen) (modLen:bnlen) = lbignum U32.(rLen +^ rLen +^ modLen +^ modLen)
 
-let get_r_i #r #m (st:rem_state r m) : lbytes r = Buffer.sub st 0ul r
-let get_tmp #r #m (st:rem_state r m) : lbytes r = Buffer.sub st r r
-let get_mod #r #m (st:rem_state r m) : lbytes m = Buffer.sub st U32.(r +^ r) m
-let get_mod_1 #r #m (st:rem_state r m) :lbytes m = Buffer.sub st U32.(r +^ r +^ m) m
+let get_r_i #r #m (st:rem_state r m) : lbignum r = Buffer.sub st 0ul r
+let get_tmp #r #m (st:rem_state r m) : lbignum r = Buffer.sub st r r
+let get_mod #r #m (st:rem_state r m) : lbignum m = Buffer.sub st U32.(r +^ r) m
+let get_mod_1 #r #m (st:rem_state r m) :lbignum m = Buffer.sub st U32.(r +^ r +^ m) m
 
 let rem_state_inv r m (st:rem_state r m) = 
            let r_i = get_r_i st in
@@ -46,25 +46,6 @@ let rem_state_inv r m (st:rem_state r m) =
 let rem_state_st_inv (rLen:bnlen) (modLen:bnlen) (st:rem_state rLen modLen) (h:FStar.HyperStack.mem) = 
 	     rem_state_inv rLen modLen st /\ live h st
 		       
-
-[@ "substitute"]
-val remainder_r_i:
-    rLen:bnlen -> modLen:bnlen{U32.v modLen = U32.v rLen} ->
-    tmp_b:bool -> st:rem_state rLen modLen -> Stack unit 
-    	       (requires (fun h -> rem_state_st_inv rLen modLen st h))
-	       (ensures (fun h r h' -> rem_state_st_inv rLen modLen st h' /\
-			        (let tmp = get_tmp st in 
-				 let r_i = get_r_i st in
-				     modifies_2 tmp r_i h h')))
-let remainder_r_i rLen modLen tmp_b st =
-    if not tmp_b then
-	let r_i = get_r_i st in
-	let tmp = get_tmp st in
-	let mod = get_mod st in
-        sub rLen modLen r_i mod tmp;
-        blit tmp 0ul r_i 0ul rLen
-
-
 val remainder_loop:
     rLen:bnlen -> modLen:bnlen{ U32.v modLen = U32.v rLen} ->
     count:U32.t ->  st:rem_state rLen modLen -> Stack unit
@@ -81,51 +62,41 @@ let rec remainder_loop rLen modLen count st =
     let mod = get_mod st in
     rshift1 modLen mod mod_1;
     let tmp_b = isMore modLen rLen mod r_i in
-    remainder_r_i rLen modLen tmp_b st;
+    (if not tmp_b then
+        (sub rLen modLen r_i mod tmp;
+        blit tmp 0ul r_i 0ul rLen));
     blit mod_1 0ul mod 0ul modLen;
     remainder_loop rLen modLen U32.(count -^ 1ul) st 
-    end 
-
-
-val remainder_:
-    rLen:bnlen ->  modLen:bnlen{U32.v modLen = U32.v rLen} ->
-    count:U32.t ->  st:rem_state rLen modLen -> Stack unit
-    (requires (fun h -> rem_state_st_inv rLen modLen st h))
-    (ensures (fun h0 _ h1 -> rem_state_st_inv rLen modLen st h1 /\ 
-			   modifies_1 st h0 h1))
-
-let remainder_ rLen modLen count st =
-    remainder_loop rLen modLen count st
+    end
 
 (* res = a % mod *)
 val remainder:
-    aBits:U32.t{U32.v aBits > 0} ->
-    modBits:U32.t{U32.v modBits > 0 /\ U32.v aBits >= U32.v modBits} ->
-    resLen:U32.t{U32.v resLen > 0} ->
-    a:bignum{length a = U32.v (bits_to_bn aBits)} ->
-    mod:bignum{length mod = U32.v (bits_to_bn modBits) /\ length mod <= length a /\ disjoint a mod} ->
-    res:bignum{length res = U32.v resLen /\ length res <= length mod /\ disjoint a res} -> Stack unit
+    aLen:bnlen ->
+    modLen:bnlen{U32.v modLen <= U32.v aLen} ->
+    resLen:bnlen{U32.v resLen <= U32.v modLen} ->
+    diffBits:U32.t{U32.v diffBits = op_Multiply 64 (U32.v aLen - U32.v modLen)} ->
+    a:lbignum aLen -> mod:lbignum modLen{disjoint a mod} ->
+    res:lbignum resLen{disjoint a res /\ disjoint mod res} -> Stack unit
 	(requires (fun h -> live h a /\ live h mod /\ live h res))
 	(ensures (fun h0 _ h1 -> live h0 a /\ live h0 mod /\  live h0 res /\
         live h1 a /\ live h1 mod /\ live h1 res /\ modifies_1 res h0 h1))
 
 #set-options "--z3rlimit 150"
 
-let remainder aBits modBits resLen a mod res =
+let remainder aLen modLen resLen diffBits a mod res =
     push_frame();
-    let aLen = bits_to_bn aBits in
-    let modLen = bits_to_bn modBits in
-    let k = U32.(aBits -^ modBits) in
-    let modk = U32.(k /^ 64ul) in
+    let modk = U32.(diffBits /^ 64ul) in
     let mod1Len = U32.(modLen +^ modk +^ 1ul) in
+    assume(U32.v mod1Len > 0 /\ U32.v mod1Len <= 8192);
     let a1Len = U32.(aLen +^ 1ul) in
+    assume(U32.v a1Len > 0 /\ U32.v a1Len <= 8192);
     let mod1Len: bnlen = mod1Len in
     let a1Len: bnlen = a1Len in
     let st : rem_state a1Len mod1Len = create 0uL U32.(a1Len +^ a1Len +^ mod1Len +^ mod1Len) in
-    let mod1 = get_mod_1 st in 
+    let mod1 = get_mod_1 st in
     let r_0 = get_r_i st in
-    lshift modLen mod k mod1;
+    lshift modLen mod diffBits mod1;
     blit a 0ul r_0 1ul aLen;
-    remainder_ a1Len mod1Len k st;
+    remainder_loop a1Len mod1Len diffBits st;
     blit r_0 0ul res 0ul resLen;
     pop_frame()
